lib/Monad_WP/NonDetMonadVCG.thy
@@ -548,6 +548,10 @@ lemma hoare_gen_asm:
   "(P \<Longrightarrow> \<lbrace>P'\<rbrace> f \<lbrace>Q\<rbrace>) \<Longrightarrow> \<lbrace>P' and K P\<rbrace> f \<lbrace>Q\<rbrace>"
   by (fastforce simp add: valid_def)
 
+lemma hoare_gen_asm_lk:
+  "(P \<Longrightarrow> \<lbrace>P'\<rbrace> f \<lbrace>Q\<rbrace>) \<Longrightarrow> \<lbrace>K P and P'\<rbrace> f \<lbrace>Q\<rbrace>"
+  by (fastforce simp add: valid_def)
+
 lemma hoare_when_wp [wp]:
  "\<lbrakk> P \<Longrightarrow> \<lbrace>Q\<rbrace> f \<lbrace>R\<rbrace> \<rbrakk> \<Longrightarrow> \<lbrace>if P then Q else R ()\<rbrace> when P f \<lbrace>R\<rbrace>"
   by (clarsimp simp: when_def valid_def return_def)
